moving toString around

thy/Iptables_Semantics/Primitive_Matchers/Code_Interface.thy
@@ -21,6 +21,11 @@ begin
 
 section\<open>Code Interface\<close>
 
+text\<open>HACK: rewrite quotes such that they are better printable by Isabelle\<close>
+definition quote_rewrite :: "string \<Rightarrow> string" where
+  "quote_rewrite \<equiv> map (\<lambda>c. if c = Char Nibble2 Nibble2 then CHR ''~'' else c)"
+
+lemma "quote_rewrite (''foo''@[Char Nibble2 Nibble2]) = ''foo~''" by eval
 
 text\<open>The parser returns the @{typ "'i::len common_primitive ruleset"} not as a map but as an association list.
       This function converts it\<close>
